coq/theories/assembly/ASMProperties.v
@@ -1,0 +1,121 @@
+Require Import impboot.utils.Core.
+Require Import impboot.utils.Llist.
+Import Llist.
+Require Import impboot.utils.Env.
+Require Import impboot.utils.AppList.
+Require Import coqutil.Word.Interface.
+Require Import impboot.assembly.ASMSyntax.
+Require Import impboot.assembly.ASMSemantics.
+
+Require Import Stdlib.Program.Equality.
+
+Require Import Patat.Patat.
+Ltac cleanup :=
+  repeat match goal with
+  | [ H: _ /\ _ |- _ ] => destruct H
+  | [ H: exists _, _ |- _ ] => destruct H
+  | [ H: True |- _ ] => clear H
+  | [ H: Some _ = Some _ |- _ ] => inversion H; subst; clear H
+  | [ H: None = Some _ |- _ ] => inversion H; subst; clear H
+  | [ H: Some _ = None |- _ ] => inversion H; subst; clear H
+  | [ H: (_, _) = (_, _) |- _ ] => inversion H; subst; clear H
+  | [ H: _ :: _ = _ :: _ |- _ ] => inversion H; subst; clear H
+  | [ H: False |- _ ] => inversion H
+  end.
+
+Lemma map_uninit_eq: forall {A B} (xs: list A) (ys: list B),
+  List.length xs = List.length ys ->
+  map (fun _ => Uninit) xs = map (fun _ => Uninit) ys.
+Proof.
+  induction xs; destruct ys; intros; simpl in *; try reflexivity; try congruence.
+  f_equal; eauto.
+Qed.
+
+Theorem step_determ: forall x y z,
+  step x y ∧ step x z -> y = z.
+Proof.
+  destruct x; intros; destruct H as [Hstep1 Hstep2].
+  2: inversion Hstep1.
+  inversion Hstep1; inversion Hstep2; subst; try reflexivity; try congruence.
+  all: pat `fetch s = _` at rewrite pat in *; cleanup.
+  - destruct yes; destruct yes0; eauto.
+    all: do 2 spat `take_branch` at inversion spat; subst; cleanup.
+    all: pat `regs s r1 = _` at rewrite pat in *; cleanup.
+    all: pat `regs s r2 = _` at rewrite pat in *; cleanup.
+    all: rewrite ?Z.ltb_lt, ?Z.ltb_ge in *.
+    all: lia.
+  - pat `stack s = _` at rewrite pat in *; cleanup.
+    pat `?xs ++ _ = _ ++ _` at eapply f_equal with (f := (fun l => skipn (List.length xs) l)) in pat.
+    rewrite skipn_app, Nat.sub_diag, skipn_all in *; simpl in *.
+    pat `List.length _ = _` at rewrite pat in *; cleanup.
+    rewrite skipn_app, Nat.sub_diag, skipn_all in *; simpl in *.
+    subst; eauto.
+  - assert (map (fun _ => Uninit) xs = map (fun _ => Uninit) xs0) as ->; eauto.
+    eapply map_uninit_eq; eauto.
+Qed.
+
+Theorem steps_determ_Halt: forall s fuel s1 s2 e1 e2 o1 o2,
+  steps (s, fuel) (Halt e1 o1, s1) ->
+  steps (s, fuel) (Halt e2 o2, s2) ->
+  e1 = e2 /\ o1 = o2.
+Proof.
+Admitted.
+
+(* TODO: share the following with ImpToAsmCodegenProof  *)
+Theorem substring_noop: forall s,
+  substring 0 (length s) s = s.
+Proof.
+  induction s.
+  - simpl; reflexivity.
+  - simpl; f_equal; assumption.
+Qed.
+Theorem prefix_refl: forall o,
+  prefix o o = true.
+Proof.
+  intros; eapply prefix_correct; eapply substring_noop.
+Qed.
+Theorem prefix_trans: forall s1 s2 s3,
+  prefix s1 s2 = true ->
+  prefix s2 s3 = true ->
+  prefix s1 s3 = true.
+Proof.
+  intros s1 s2. revert s1.
+  induction s2 as [|b s2' IH]; intros s1 s3 H1 H2.
+  - destruct s1 as [|a s1'].
+    + simpl. assumption.
+    + simpl in H1. discriminate H1.
+  - destruct s1 as [|a s1'].
+    + destruct s3 as [|c s3']; simpl; reflexivity.
+    + simpl in H1.
+      destruct (ascii_dec a b) as [Heq|Hneq].
+      * subst b.
+        destruct s3 as [|c s3'].
+        -- simpl in H2.
+           destruct (ascii_dec a a) as [_|Hcontr]; [discriminate H2|contradiction].
+        -- simpl in H2.
+           destruct (ascii_dec a c) as [Heq2|Hneq2].
+           ++ subst c.
+              simpl.
+              destruct (ascii_dec a a) as [_|Hcontr]; [|contradiction].
+              eapply IH; eassumption.
+           ++ discriminate H2.
+      * discriminate H1.
+Qed.
+Lemma substring_append: forall (s s1: string),
+  substring 0 (length s) (s ++ s1) = s.
+Proof.
+  induction s; simpl; intros.
+  - destruct s1; simpl; reflexivity.
+  - f_equal; eauto.
+Qed.
+
+Theorem step_mono: forall s0 s1,
+  step (State s0) (State s1) -> prefix s0.(output) s1.(output) = true.
+Proof.
+  inversion 1; intros; subst; simpl.
+  all: try eapply prefix_refl.
+  1: unfold write_mem in *; spat `match ?c with _ => _ end` at destruct c eqn:?; cleanup; simpl.
+  1: eapply prefix_refl.
+  eapply prefix_correct.
+  rewrite substring_append; reflexivity.
+Qed.
